@prefix : <http://ld.nice.org.uk/ns/qualitystandard/setting#> .
@prefix owl: <http://www.w3.org/2002/07/owl#> .
@prefix rdf: <http://www.w3.org/1999/02/22-rdf-syntax-ns#> .
@prefix xml: <http://www.w3.org/XML/1998/namespace> .
@prefix xsd: <http://www.w3.org/2001/XMLSchema#> .
@prefix rdfs: <http://www.w3.org/2000/01/rdf-schema#> .
@base <http://ld.nice.org.uk/ns/qualitystandard/setting> .

<http://ld.nice.org.uk/ns/qualitystandard/setting> rdf:type owl:Ontology ;
                                                    owl:imports <http://www.w3.org/2004/02/skos/core> .

#################################################################
#    Classes
#################################################################

###  http://ld.nice.org.uk/ns/qualitystandard/setting#ad41399f_826e_427f_840a_2cb36ee22d92
:ad41399f_826e_427f_840a_2cb36ee22d92 rdf:type owl:Class ;
                                      rdfs:subClassOf :6f40063c_702a_4101_ab21_516b74a38519 ;
                                      rdfs:label "Hospice"@en ;
                                      <http://www.w3.org/2004/02/skos/core#definition> "To include inpatient and day hospices."@en ;
                                      <http://www.w3.org/2004/02/skos/core#prefLabel> "Hospice"@en .


###  http://ld.nice.org.uk/ns/qualitystandard/setting#e517e9af_3c12_4f8b_a320_9323dfdf2510
:e517e9af_3c12_4f8b_a320_9323dfdf2510 rdf:type owl:Class ;
                                      rdfs:subClassOf :6f40063c_702a_4101_ab21_516b74a38519 ;
                                      rdfs:label "Community"@en ;
                                      <http://www.w3.org/2004/02/skos/core#definition> "To include schools, workplaces, in the home, supported living."@en ;
                                      <http://www.w3.org/2004/02/skos/core#prefLabel> "Community"@en .


###  http://ld.nice.org.uk/ns/qualitystandard/setting#f023a36e_2b46_40ae_b775_241126ab76bd
:f023a36e_2b46_40ae_b775_241126ab76bd rdf:type owl:Class ;
                                      rdfs:subClassOf :6f40063c_702a_4101_ab21_516b74a38519 ;
                                      rdfs:label "Care home"@en ;
                                      <http://www.w3.org/2004/02/skos/core#altLabel> "Nursing home"@en ,
                                                                                     "Rest home"@en ;
                                      <http://www.w3.org/2004/02/skos/core#definition> "To include all homes (both residential care and nursing  homes) that offer accommodation and personal care and support for  adults or children who may not be able to live independently."@en ;
                                      <http://www.w3.org/2004/02/skos/core#prefLabel> "Care home"@en .


###  http://ld.nice.org.uk/ns/qualitystandard/setting#16764614_b99f_401e_b95c_d9721dd20825
:16764614_b99f_401e_b95c_d9721dd20825 rdf:type owl:Class ;
                                      rdfs:subClassOf :6f40063c_702a_4101_ab21_516b74a38519 ;
                                      rdfs:label "Outpatient clinic"@en ;
                                      <http://www.w3.org/2004/02/skos/core#altLabel> "Outpatient department"@en ;
                                      <http://www.w3.org/2004/02/skos/core#definition> "To include outpatient clinics providing specialist secondary medical and mental health outpatient services that may or may not be attached to hospital."@en ;
                                      <http://www.w3.org/2004/02/skos/core#prefLabel> "Outpatient clinic"@en .


###  http://ld.nice.org.uk/ns/qualitystandard/setting#6f40063c_702a_4101_ab21_516b74a38519
:6f40063c_702a_4101_ab21_516b74a38519 rdf:type owl:Class ;
                                      rdfs:label "Setting"@en ;
                                      <http://www.w3.org/2004/02/skos/core#prefLabel> "Setting"@en .


###  http://ld.nice.org.uk/ns/qualitystandard/setting#6369f927_a7b7_42ba_bf68_39482e32d7ab
:6369f927_a7b7_42ba_bf68_39482e32d7ab rdf:type owl:Class ;
                                      rdfs:subClassOf :6f40063c_702a_4101_ab21_516b74a38519 ;
                                      rdfs:label "Hospital"@en ;
                                      <http://www.w3.org/2004/02/skos/core#altLabel> "Inpatient"@en ,
                                                                                     "Ward"@en ;
                                      <http://www.w3.org/2004/02/skos/core#definition> "To include acute, community and mental health hospitals providing inpatient services."@en ;
                                      <http://www.w3.org/2004/02/skos/core#prefLabel> "Hospital"@en .


###  http://ld.nice.org.uk/ns/qualitystandard/setting#80c545e4_a13c_4373_a530_18f0239ce548
:80c545e4_a13c_4373_a530_18f0239ce548 rdf:type owl:Class ;
                                      rdfs:subClassOf :6f40063c_702a_4101_ab21_516b74a38519 ;
                                      rdfs:label "Primary care setting"@en ;
                                      <http://www.w3.org/2004/02/skos/core#definition> "To include GP practices, dental surgeries, optometrists, community pharmacies."@en ;
                                      <http://www.w3.org/2004/02/skos/core#prefLabel> "Primary care setting"@en .


###  Generated by the OWL API (version 4.2.5.20160517-0735) https://github.com/owlcs/owlapi
