@prefix : <http://ld.nice.org.uk/ns/qualitystandard/setting#> .
@prefix owl: <http://www.w3.org/2002/07/owl#> .
@prefix rdf: <http://www.w3.org/1999/02/22-rdf-syntax-ns#> .
@prefix xml: <http://www.w3.org/XML/1998/namespace> .
@prefix xsd: <http://www.w3.org/2001/XMLSchema#> .
@prefix rdfs: <http://www.w3.org/2000/01/rdf-schema#> .

<http://ld.nice.org.uk/ns/qualitystandard/setting> a owl:Ontology ;
	owl:imports <http://www.w3.org/2004/02/skos/core> .
# 
# 
# #################################################################
# #
# #    Classes
# #
# #################################################################
# 
# 
# http://ld.nice.org.uk/ns/qualitystandard/setting#CareHome

:CareHome a owl:Class ;
	rdfs:subClassOf :Setting ;
	rdfs:label "Care home"@en ;
	<http://www.w3.org/2004/02/skos/core#altLabel> "Nursing home"@en , "Rest home"@en ;
	<http://www.w3.org/2004/02/skos/core#definition> "To include all homes (both residential care and nursing  homes) that offer accommodation and personal care and support for  adults or children who may not be able to live independently."@en ;
	<http://www.w3.org/2004/02/skos/core#prefLabel> "Care home"@en .
# 
# http://ld.nice.org.uk/ns/qualitystandard/setting#Community

:Community a owl:Class ;
	rdfs:subClassOf :Setting ;
	rdfs:label "Community"@en ;
	<http://www.w3.org/2004/02/skos/core#definition> "To include schools, workplaces, in the home, supported living."@en ;
	<http://www.w3.org/2004/02/skos/core#prefLabel> "Community"@en .
# 
# http://ld.nice.org.uk/ns/qualitystandard/setting#Hospice

:Hospice a owl:Class ;
	rdfs:subClassOf :Setting ;
	rdfs:label "Hospice"@en ;
	<http://www.w3.org/2004/02/skos/core#definition> "To include inpatient and day hospices."@en ;
	<http://www.w3.org/2004/02/skos/core#prefLabel> "Hospice"@en .
# 
# http://ld.nice.org.uk/ns/qualitystandard/setting#Hospital

:Hospital a owl:Class ;
	rdfs:subClassOf :Setting ;
	rdfs:label "Hospital"@en ;
	<http://www.w3.org/2004/02/skos/core#altLabel> "Inpatient"@en , "Ward"@en ;
	<http://www.w3.org/2004/02/skos/core#definition> "To include acute, community and mental health hospitals providing inpatient services."@en ;
	<http://www.w3.org/2004/02/skos/core#prefLabel> "Hospital"@en .
# 
# http://ld.nice.org.uk/ns/qualitystandard/setting#OutpatientClinic

:OutpatientClinic a owl:Class ;
	rdfs:subClassOf :Setting ;
	rdfs:label "Outpatient clinic"@en ;
	<http://www.w3.org/2004/02/skos/core#altLabel> "Outpatient department"@en ;
	<http://www.w3.org/2004/02/skos/core#definition> "To include outpatient clinics providing specialist secondary medical and mental health outpatient services that may or may not be attached to hospital."@en ;
	<http://www.w3.org/2004/02/skos/core#prefLabel> "Outpatient clinic"@en .
# 
# http://ld.nice.org.uk/ns/qualitystandard/setting#PrimaryCareSetting

:PrimaryCareSetting a owl:Class ;
	rdfs:subClassOf :Setting ;
	rdfs:label "Primary care setting"@en ;
	<http://www.w3.org/2004/02/skos/core#definition> "To include GP practices, dental surgeries, optometrists, community pharmacies."@en ;
	<http://www.w3.org/2004/02/skos/core#prefLabel> "Primary care setting"@en .
# 
# http://ld.nice.org.uk/ns/qualitystandard/setting#Setting

:Setting a owl:Class ;
	rdfs:label "Setting"@en ;
	<http://www.w3.org/2004/02/skos/core#prefLabel> "Setting"@en .
# 
# Generated by the OWL API (version 4.2.5.20160517-0735) https://github.com/owlcs/owlapi
