Prefix: : <http://ld.nice.org.uk/ns/qualitystandard#>
Prefix: dc: <http://purl.org/dc/elements/1.1/>
Prefix: owl: <http://www.w3.org/2002/07/owl#>
Prefix: rdf: <http://www.w3.org/1999/02/22-rdf-syntax-ns#>
Prefix: xml: <http://www.w3.org/XML/1998/namespace>
Prefix: xsd: <http://www.w3.org/2001/XMLSchema#>
Prefix: pico: <http://ld.nice.org.uk/ns/pico#>
Prefix: rdfs: <http://www.w3.org/2000/01/rdf-schema#>
Prefix: skos: <http://www.w3.org/2004/02/skos/core#>
Prefix: setting: <http://ld.nice.org.uk/ns/qualitystandard/setting#>
Prefix: agegroup: <http://ld.nice.org.uk/ns/qualitystandard/agegroup#>
Prefix: servicearea: <http://ld.nice.org.uk/ns/qualitystandard/servicearea#>
Prefix: conditionordisease: <http://ld.nice.org.uk/ns/qualitystandard/conditionordisease#>
Prefix: lifestylecondition: <http://ld.nice.org.uk/ns/qualitystandard/lifestylecondition#>



Ontology: <http://www.w3.org/2004/02/skos/core#closeMatch>


AnnotationProperty: rdfs:isDefinedBy

    
AnnotationProperty: skos:prefLabel

    Annotations: 
        rdfs:comment "Should be the same as the class label"
    
    Annotations: 
        rdfs:comment "Should be the same as the class label"
    
    
AnnotationProperty: <http://ld.nice.org.uk/ns/qualitystandard#include_drug_abuse,_alcohol_abuse,_obesity>

    SubPropertyOf: 
        rdfs:comment
    
    
AnnotationProperty: rdfs:comment

    
AnnotationProperty: skos:altLabel

    Annotations: 
        rdfs:comment "Use for synonyms"
    
    Annotations: 
        rdfs:comment "Use for synonyms"
    
    
Datatype: xsd:dateTime

    
Datatype: rdfs:Literal

    
Datatype: xsd:integer

    
Datatype: xsd:string

    
Datatype: rdf:PlainLiteral

    
ObjectProperty: condition

    Domain: 
        pico:Population
    
    Range: 
        conditionordisease:ConditionOrDisease
    
    
ObjectProperty: lifestyleCondition

    Domain: 
        pico:Population
    
    Range: 
        lifestylecondition:LifestyleCondition
    
    
ObjectProperty: definesTask

    Annotations: 
        rdfs:comment "Connects  proposed action of quality statement to tasks which enable this action to take place"
    
    Domain: 
        QualityStatement
    
    SubPropertyOf: 
        owl:topObjectProperty
    
    InverseOf: 
        definedTaskOf
    
    
ObjectProperty: replacedBy

    Domain: 
        owl:Thing
    
    Range: 
        owl:Thing
    
    InverseOf: 
        replaces
    
    
ObjectProperty: taskOwner

    InverseOf: 
        ownsTask
    
    
ObjectProperty: hasPart

    Characteristics: 
        Transitive
    
    InverseOf: 
        partOf
    
    
ObjectProperty: hasConcept

    InverseOf: 
        skos:inConceptScheme
    
    
ObjectProperty: measuresProgressAgainst

    Domain: 
        QualityMeasure
    
    
ObjectProperty: replaces

    Domain: 
        owl:Thing
    
    Range: 
        owl:Thing
    
    InverseOf: 
        replacedBy
    
    
ObjectProperty: isSpecifiedBy

    Domain: 
        pico:Population
    
    Range: 
        PopulationSpecifier
    
    InverseOf: 
        specifies
    
    
ObjectProperty: hasGuidanceStatus

    Domain: 
        owl:Thing
    
    Range: 
        GuidanceStatus
    
    
ObjectProperty: isServiceAreaOf

    Domain: 
        servicearea:ServiceArea
    
    Range: 
        QualityStatement
    
    InverseOf: 
        serviceArea
    
    
ObjectProperty: owl:topObjectProperty

    
ObjectProperty: definesMeasure

    Annotations: 
        rdfs:comment "one quality statement may hve several measures associated with it."
    
    Domain: 
        QualityStatement
    
    Range: 
        QualityMeasure
    
    InverseOf: 
        measureDefinedBy
    
    
ObjectProperty: isTargetPopulationOf

    Domain: 
        pico:Population
    
    Range: 
        QualityStatement
    
    SubPropertyOf: 
        owl:topObjectProperty
    
    InverseOf: 
        targetPopulation
    
    
ObjectProperty: age

    Annotations: 
        rdfs:comment "Defines age profile of target population by linking to age group"
    
    Domain: 
        pico:Population
    
    Range: 
        agegroup:AgeGroup
    
    
ObjectProperty: haschangeLog

    Domain: 
        owl:Thing
    
    Range: 
        ChangeLog
    
    
ObjectProperty: skos:inConceptScheme

    InverseOf: 
        hasConcept
    
    
ObjectProperty: ownsTask

    InverseOf: 
        taskOwner
    
    
ObjectProperty: serviceArea

    Annotations: 
        rdfs:comment "links a quality statement to service area that  the statement is applicable to."
    
    Domain: 
        QualityStatement
    
    Range: 
        servicearea:ServiceArea
    
    InverseOf: 
        isServiceAreaOf
    
    
ObjectProperty: measureDefinedBy

    Domain: 
        QualityMeasure
    
    Range: 
        QualityStatement
    
    InverseOf: 
        definesMeasure
    
    
ObjectProperty: haschangeType

    Domain: 
        owl:Thing
    
    Range: 
        ChangeType
    
    
ObjectProperty: haschangeEntry

    Domain: 
        ChangeLog
    
    Range: 
        ChangeEntry
    
    
ObjectProperty: partOf

    Characteristics: 
        Transitive
    
    InverseOf: 
        hasPart
    
    
ObjectProperty: skos:closeMatch

    Annotations: 
        rdfs:comment "To be used for mapping to  external ontology concepts e.g. SNOMED"
    
    Domain: 
        conditionordisease:ConditionOrDisease
    
    
ObjectProperty: targetPopulation

    Annotations: 
        rdfs:comment "Links a quality statement with the target population for which the statement is applicable"
    
    Domain: 
        QualityStatement
    
    Range: 
        pico:Population
    
    InverseOf: 
        isTargetPopulationOf
    
    
ObjectProperty: specifies

    Domain: 
        PopulationSpecifier
    
    Range: 
        pico:Population
    
    InverseOf: 
        isSpecifiedBy
    
    
ObjectProperty: setting

    Annotations: 
        rdfs:comment "Links a quality statement to a physical setting that the statement is applicable to."
    
    Domain: 
        QualityStatement
    
    Range: 
        setting:Setting
    
    InverseOf: 
        isSettingOf
    
    
ObjectProperty: definedTaskOf

    Range: 
        QualityStatement
    
    InverseOf: 
        definesTask
    
    
ObjectProperty: isSettingOf

    Domain: 
        setting:Setting
    
    Range: 
        QualityStatement
    
    InverseOf: 
        setting
    
    
DataProperty: hasDataSource

    Domain: 
        QualityMeasure
    
    Range: 
        rdfs:Literal
    
    
DataProperty: <http://purl.org/dc/terms/identifier>

    Annotations: 
        rdfs:comment "An unambiguous reference to the resource within a given context.",
        rdfs:isDefinedBy <http://purl.org/dc/terms>
    
    Domain: 
        Product
    
    Range: 
        xsd:integer
    
    
DataProperty: <http://purl.org/dc/terms/date>

    
DataProperty: dateIssued

    Annotations: 
        rdfs:isDefinedBy "<http://purl.org/dc/terms/>",
        rdfs:comment "Date of formal issuance (e.g., publication) of the resource."
    
    Domain: 
        owl:Thing
    
    Range: 
        xsd:dateTime
    
    SubPropertyOf: 
        <http://purl.org/dc/terms/date>
    
    
DataProperty: dateModified

    Annotations: 
        rdfs:isDefinedBy "<http://purl.org/dc/terms/>",
        rdfs:comment "Date on which the resource was changed."
    
    Domain: 
        owl:Thing
    
    Range: 
        xsd:dateTime
    
    SubPropertyOf: 
        <http://purl.org/dc/terms/date>
    
    
DataProperty: <http://purl.org/dc/terms/abstract>

    Annotations: 
        rdfs:isDefinedBy <http://purl.org/dc/terms>,
        rdfs:comment "A summary of the resource."
    
    Domain: 
        owl:Thing
    
    Range: 
        xsd:string
    
    
DataProperty: <http://purl.org/dc/terms/title>

    Annotations: 
        rdfs:isDefinedBy "http://purl.org/dc/terms",
        rdfs:comment "A name given to the resource."
    
    Domain: 
        owl:Thing
    
    Range: 
        xsd:string
    
    
DataProperty: <http://ld.nice.org.uk/ns/qualitystandard#qs::hasNumerator>

    Domain: 
        ProcessMeasure
    
    Range: 
        xsd:string
    
    
DataProperty: <http://ld.nice.org.uk/ns/qualitystandard#qs::hasDenominator>

    Domain: 
        QualityMeasure
    
    Range: 
        xsd:string
    
    
DataProperty: haschangeSummary

    Domain: 
        owl:Thing
    
    Range: 
        xsd:string
    
    
DataProperty: dateWithdrawn

    Annotations: 
        rdfs:comment "Date on which the resource was withdrawn."
    
    Domain: 
        owl:Thing
    
    Range: 
        xsd:dateTime
    
    SubPropertyOf: 
        <http://purl.org/dc/terms/date>
    
    
DataProperty: haschangeDescription

    Domain: 
        owl:Thing
    
    Range: 
        xsd:string
    
    
Class: Product

    
Class: QualityMeasure

    Annotations: 
        rdfs:comment "Quality measures are used to assess the quality of care or service provision specified in the quality statement."
    
    
Class: TopLevelProvenanceConcept

    
Class: conditionordisease:ConditionOrDisease

    Annotations: 
        rdfs:comment "Class of conditions and diseases for population specification. Top level based on NICE Browse taxonomy structure. Mapping to equivalent SNOMED code where possible. Used for medical and mental health conditions."
    
    SubClassOf: 
        PopulationSpecifier
    
    
Class: agegroup:AgeGroup

    Annotations: 
        rdfs:comment "List of age groups to support population definition."
    
    SubClassOf: 
        PopulationSpecifier
    
    
Class: OutcomeMeasure

    Annotations: 
        rdfs:comment "An outcome measure addresses the outcome of care or service provision."
    
    SubClassOf: 
        QualityMeasure
    
    DisjointWith: 
        ProcessMeasure, StructureMeasure
    
    
Class: QualityStandard

    Annotations: 
        rdfs:comment "NICE quality standards are concise sets of prioritised  quality statements designed to drive measurable quality improvements within a particular area of health or care."
    
    SubClassOf: 
        Product,
        hasPart some QualityStatement
    
    DisjointWith: 
        QualityStatement
    
    
Class: Published

    Annotations: 
        rdfs:comment "Status of a resource that has been published and has not been withdrawn (still valid)."
    
    SubClassOf: 
        dateIssued some xsd:dateTime,
        dateWithdrawn max 0 xsd:dateTime,
        GuidanceStatus
    
    DisjointWith: 
        Withdrawn
    
    
Class: owl:Thing

    
Class: ChangeLog

    SubClassOf: 
        TopLevelProvenanceConcept,
        haschangeEntry min 1 ChangeEntry
    
    
Class: PopulationSpecifier

    Annotations: 
        rdfs:comment "A class of facets by which a target population can be specified."
    
    
Class: StructureMeasure

    Annotations: 
        rdfs:comment "A  structure measure addresses the structure of care or services."
    
    SubClassOf: 
        QualityMeasure
    
    DisjointWith: 
        ProcessMeasure, OutcomeMeasure
    
    
Class: GuidanceStatus

    Annotations: 
        rdfs:comment "The publication status of a NICE resource."
    
    
Class: MajorChange

    SubClassOf: 
        ChangeType
    
    DisjointWith: 
        MinorChange
    
    
Class: Withdrawn

    Annotations: 
        rdfs:comment "Status of a resource that thas been withdrawn after some time when it was a valid, published resource. No longer valid."
    
    SubClassOf: 
        GuidanceStatus,
        dateWithdrawn some xsd:dateTime
    
    DisjointWith: 
        Published
    
    
Class: QualityStatement

    Annotations: 
        rdfs:comment "A NICE Quality statement is a clear, measurable and concise statement to describe ‘enhanced practice’, which is both aspirational and achievable."
    
    SubClassOf: 
        Product,
        partOf some QualityStandard
    
    DisjointWith: 
        QualityStandard
    
    
Class: ProcessMeasure

    Annotations: 
        rdfs:comment "A process measure addresses the process of care or service provision"
    
    SubClassOf: 
        QualityMeasure
    
    DisjointWith: 
        StructureMeasure, OutcomeMeasure
    
    
Class: lifestylecondition:LifestyleCondition

    Annotations: 
        rdfs:comment "Conditions which have associated lifestyle factors, to include drug abuse, alcohol abuse and diet and physical activity related conditions."
    
    SubClassOf: 
        PopulationSpecifier
    
    
Class: PlaceholderStatement

    Annotations: 
        rdfs:comment "A placeholder statement is an area of care that has been prioritised by the Quality Standards Advisory Committee but for which no source guidance is currently available. A placeholder statement indicates the need for evidence‑based guidance to be developed in this area."
    
    
Class: MinorChange

    SubClassOf: 
        ChangeType
    
    DisjointWith: 
        MajorChange
    
    
Class: ChangeEntry

    SubClassOf: 
        haschangeDescription some xsd:string,
        haschangeType exactly 1 ChangeType,
        TopLevelProvenanceConcept,
        haschangeSummary some xsd:string
    
    
Class: pico:Population

    Annotations: 
        rdfs:comment "Defined by at least one of the age, gender, ethnicity, disease, lifestyle condition concepts."
    
    EquivalentTo: 
        isSpecifiedBy min 1 PopulationSpecifier
    
    
Class: servicearea:ServiceArea

    Annotations: 
        rdfs:comment "Health or care service area to which a NICE quality statement is applicable."
    
    
Class: setting:Setting

    Annotations: 
        rdfs:comment "Physical setting  to which NICE quality statement is applicable."
    
    
Class: ChangeType

    SubClassOf: 
        TopLevelProvenanceConcept
    
    
Class: DevelopmentalQualityStatement

    Annotations: 
        rdfs:comment "A developmental quality statement sets out an emergent area of cutting‑edge service delivery or technology currently found in a minority of providers and indicating outstanding performance. It will require specific, significant changes to be put in place, such as redesign of services or new equipment."
    
    SubClassOf: 
        QualityStatement
    
    
