Prefix: : <http://ld.nice.org.uk/ns/qualitystandard/>
Prefix: agegroup: <http://ld.nice.org.uk/ns/qualitystandard/agegroup#>
Prefix: conditionordisease: <http://ld.nice.org.uk/ns/qualitystandard/conditionordisease#>
Prefix: dc: <http://purl.org/dc/elements/1.1/>
Prefix: lifestylecondition: <http://ld.nice.org.uk/ns/qualitystandard/lifestylecondition#>
Prefix: owl: <http://www.w3.org/2002/07/owl#>
Prefix: pico: <http://ld.nice.org.uk/ns/pico#>
Prefix: rdf: <http://www.w3.org/1999/02/22-rdf-syntax-ns#>
Prefix: rdfs: <http://www.w3.org/2000/01/rdf-schema#>
Prefix: servicearea: <http://ld.nice.org.uk/ns/qualitystandard/servicearea#>
Prefix: setting: <http://ld.nice.org.uk/ns/qualitystandard/setting#>
Prefix: skos: <http://www.w3.org/2004/02/skos/core#>
Prefix: xml: <http://www.w3.org/XML/1998/namespace>
Prefix: xsd: <http://www.w3.org/2001/XMLSchema#>



Ontology: <http://ld.nice.org.uk/ns/qualitystandard>


AnnotationProperty: <http://ld.nice.org.uk/ns/qualitystandard#include_drug_abuse,_alcohol_abuse,_obesity>

    SubPropertyOf: 
        rdfs:comment
    
    
AnnotationProperty: rdfs:comment

    
AnnotationProperty: rdfs:isDefinedBy

    
AnnotationProperty: skos:altLabel

    Annotations: 
        rdfs:comment "Use for synonyms"
    
    
AnnotationProperty: skos:prefLabel

    Annotations: 
        rdfs:comment "Should be the same as the class label"
    
    
Datatype: rdf:PlainLiteral

    
Datatype: rdfs:Literal

    
Datatype: xsd:dateTime

    
Datatype: xsd:integer

    
Datatype: xsd:string

    
ObjectProperty: <http://ld.nice.org.uk/ns/qualitystandard#age>

    Annotations: 
        rdfs:comment "Defines age profile of target population by linking to age group"
    
    Domain: 
        pico:Population
    
    Range: 
        agegroup:AgeGroup
    
    
ObjectProperty: <http://ld.nice.org.uk/ns/qualitystandard#condition>

    Domain: 
        pico:Population
    
    Range: 
        conditionordisease:ConditionOrDisease
    
    
ObjectProperty: <http://ld.nice.org.uk/ns/qualitystandard#definedTaskOf>

    Range: 
        <http://ld.nice.org.uk/ns/qualitystandard#QualityStatement>
    
    InverseOf: 
        <http://ld.nice.org.uk/ns/qualitystandard#definesTask>
    
    
ObjectProperty: <http://ld.nice.org.uk/ns/qualitystandard#definesMeasure>

    Annotations: 
        rdfs:comment "one quality statement may hve several measures associated with it."
    
    Domain: 
        <http://ld.nice.org.uk/ns/qualitystandard#QualityStatement>
    
    Range: 
        <http://ld.nice.org.uk/ns/qualitystandard#QualityMeasure>
    
    InverseOf: 
        <http://ld.nice.org.uk/ns/qualitystandard#measureDefinedBy>
    
    
ObjectProperty: <http://ld.nice.org.uk/ns/qualitystandard#definesTask>

    Annotations: 
        rdfs:comment "Connects  proposed action of quality statement to tasks which enable this action to take place"
    
    SubPropertyOf: 
        owl:topObjectProperty
    
    Domain: 
        <http://ld.nice.org.uk/ns/qualitystandard#QualityStatement>
    
    InverseOf: 
        <http://ld.nice.org.uk/ns/qualitystandard#definedTaskOf>
    
    
ObjectProperty: <http://ld.nice.org.uk/ns/qualitystandard#hasConcept>

    InverseOf: 
        skos:inConceptScheme
    
    
ObjectProperty: <http://ld.nice.org.uk/ns/qualitystandard#hasGuidanceStatus>

    Domain: 
        owl:Thing
    
    Range: 
        <http://ld.nice.org.uk/ns/qualitystandard#GuidanceStatus>
    
    
ObjectProperty: <http://ld.nice.org.uk/ns/qualitystandard#hasPart>

    Characteristics: 
        Transitive
    
    InverseOf: 
        <http://ld.nice.org.uk/ns/qualitystandard#partOf>
    
    
ObjectProperty: <http://ld.nice.org.uk/ns/qualitystandard#haschangeEntry>

    Domain: 
        <http://ld.nice.org.uk/ns/qualitystandard#ChangeLog>
    
    Range: 
        <http://ld.nice.org.uk/ns/qualitystandard#ChangeEntry>
    
    
ObjectProperty: <http://ld.nice.org.uk/ns/qualitystandard#haschangeLog>

    Domain: 
        owl:Thing
    
    Range: 
        <http://ld.nice.org.uk/ns/qualitystandard#ChangeLog>
    
    
ObjectProperty: <http://ld.nice.org.uk/ns/qualitystandard#haschangeType>

    Domain: 
        owl:Thing
    
    Range: 
        <http://ld.nice.org.uk/ns/qualitystandard#ChangeType>
    
    
ObjectProperty: <http://ld.nice.org.uk/ns/qualitystandard#isServiceAreaOf>

    Domain: 
        servicearea:ServiceArea
    
    Range: 
        <http://ld.nice.org.uk/ns/qualitystandard#QualityStatement>
    
    InverseOf: 
        <http://ld.nice.org.uk/ns/qualitystandard#serviceArea>
    
    
ObjectProperty: <http://ld.nice.org.uk/ns/qualitystandard#isSettingOf>

    Domain: 
        setting:Setting
    
    Range: 
        <http://ld.nice.org.uk/ns/qualitystandard#QualityStatement>
    
    InverseOf: 
        <http://ld.nice.org.uk/ns/qualitystandard#setting>
    
    
ObjectProperty: <http://ld.nice.org.uk/ns/qualitystandard#isSpecifiedBy>

    Domain: 
        pico:Population
    
    Range: 
        <http://ld.nice.org.uk/ns/qualitystandard#PopulationSpecifier>
    
    InverseOf: 
        <http://ld.nice.org.uk/ns/qualitystandard#specifies>
    
    
ObjectProperty: <http://ld.nice.org.uk/ns/qualitystandard#isTargetPopulationOf>

    SubPropertyOf: 
        owl:topObjectProperty
    
    Domain: 
        pico:Population
    
    Range: 
        <http://ld.nice.org.uk/ns/qualitystandard#QualityStatement>
    
    InverseOf: 
        <http://ld.nice.org.uk/ns/qualitystandard#targetPopulation>
    
    
ObjectProperty: <http://ld.nice.org.uk/ns/qualitystandard#lifestyleCondition>

    Domain: 
        pico:Population
    
    Range: 
        lifestylecondition:LifestyleCondition
    
    
ObjectProperty: <http://ld.nice.org.uk/ns/qualitystandard#measureDefinedBy>

    Domain: 
        <http://ld.nice.org.uk/ns/qualitystandard#QualityMeasure>
    
    Range: 
        <http://ld.nice.org.uk/ns/qualitystandard#QualityStatement>
    
    InverseOf: 
        <http://ld.nice.org.uk/ns/qualitystandard#definesMeasure>
    
    
ObjectProperty: <http://ld.nice.org.uk/ns/qualitystandard#measuresProgressAgainst>

    Domain: 
        <http://ld.nice.org.uk/ns/qualitystandard#QualityMeasure>
    
    
ObjectProperty: <http://ld.nice.org.uk/ns/qualitystandard#ownsTask>

    InverseOf: 
        <http://ld.nice.org.uk/ns/qualitystandard#taskOwner>
    
    
ObjectProperty: <http://ld.nice.org.uk/ns/qualitystandard#partOf>

    Characteristics: 
        Transitive
    
    InverseOf: 
        <http://ld.nice.org.uk/ns/qualitystandard#hasPart>
    
    
ObjectProperty: <http://ld.nice.org.uk/ns/qualitystandard#replacedBy>

    Domain: 
        owl:Thing
    
    Range: 
        owl:Thing
    
    InverseOf: 
        <http://ld.nice.org.uk/ns/qualitystandard#replaces>
    
    
ObjectProperty: <http://ld.nice.org.uk/ns/qualitystandard#replaces>

    Domain: 
        owl:Thing
    
    Range: 
        owl:Thing
    
    InverseOf: 
        <http://ld.nice.org.uk/ns/qualitystandard#replacedBy>
    
    
ObjectProperty: <http://ld.nice.org.uk/ns/qualitystandard#serviceArea>

    Annotations: 
        rdfs:comment "links a quality statement to service area that  the statement is applicable to."
    
    Domain: 
        <http://ld.nice.org.uk/ns/qualitystandard#QualityStatement>
    
    Range: 
        servicearea:ServiceArea
    
    InverseOf: 
        <http://ld.nice.org.uk/ns/qualitystandard#isServiceAreaOf>
    
    
ObjectProperty: <http://ld.nice.org.uk/ns/qualitystandard#setting>

    Annotations: 
        rdfs:comment "Links a quality statement to a physical setting that the statement is applicable to."
    
    Domain: 
        <http://ld.nice.org.uk/ns/qualitystandard#QualityStatement>
    
    Range: 
        setting:Setting
    
    InverseOf: 
        <http://ld.nice.org.uk/ns/qualitystandard#isSettingOf>
    
    
ObjectProperty: <http://ld.nice.org.uk/ns/qualitystandard#specifies>

    Domain: 
        <http://ld.nice.org.uk/ns/qualitystandard#PopulationSpecifier>
    
    Range: 
        pico:Population
    
    InverseOf: 
        <http://ld.nice.org.uk/ns/qualitystandard#isSpecifiedBy>
    
    
ObjectProperty: <http://ld.nice.org.uk/ns/qualitystandard#targetPopulation>

    Annotations: 
        rdfs:comment "Links a quality statement with the target population for which the statement is applicable"
    
    Domain: 
        <http://ld.nice.org.uk/ns/qualitystandard#QualityStatement>
    
    Range: 
        pico:Population
    
    InverseOf: 
        <http://ld.nice.org.uk/ns/qualitystandard#isTargetPopulationOf>
    
    
ObjectProperty: <http://ld.nice.org.uk/ns/qualitystandard#taskOwner>

    InverseOf: 
        <http://ld.nice.org.uk/ns/qualitystandard#ownsTask>
    
    
ObjectProperty: owl:topObjectProperty

    
ObjectProperty: skos:closeMatch

    Annotations: 
        rdfs:comment "To be used for mapping to  external ontology concepts e.g. SNOMED"
    
    Domain: 
        conditionordisease:ConditionOrDisease
    
    
ObjectProperty: skos:inConceptScheme

    InverseOf: 
        <http://ld.nice.org.uk/ns/qualitystandard#hasConcept>
    
    
DataProperty: <http://ld.nice.org.uk/ns/qualitystandard#dateIssued>

    Annotations: 
        rdfs:comment "Date of formal issuance (e.g., publication) of the resource.",
        rdfs:isDefinedBy "<http://purl.org/dc/terms/>"
    
    Domain: 
        owl:Thing
    
    Range: 
        xsd:dateTime
    
    SubPropertyOf: 
        <http://purl.org/dc/terms/date>
    
    
DataProperty: <http://ld.nice.org.uk/ns/qualitystandard#dateModified>

    Annotations: 
        rdfs:comment "Date on which the resource was changed.",
        rdfs:isDefinedBy "<http://purl.org/dc/terms/>"
    
    Domain: 
        owl:Thing
    
    Range: 
        xsd:dateTime
    
    SubPropertyOf: 
        <http://purl.org/dc/terms/date>
    
    
DataProperty: <http://ld.nice.org.uk/ns/qualitystandard#dateWithdrawn>

    Annotations: 
        rdfs:comment "Date on which the resource was withdrawn."
    
    Domain: 
        owl:Thing
    
    Range: 
        xsd:dateTime
    
    SubPropertyOf: 
        <http://purl.org/dc/terms/date>
    
    
DataProperty: <http://ld.nice.org.uk/ns/qualitystandard#hasDataSource>

    Domain: 
        <http://ld.nice.org.uk/ns/qualitystandard#QualityMeasure>
    
    Range: 
        rdfs:Literal
    
    
DataProperty: <http://ld.nice.org.uk/ns/qualitystandard#haschangeDescription>

    Domain: 
        owl:Thing
    
    Range: 
        xsd:string
    
    
DataProperty: <http://ld.nice.org.uk/ns/qualitystandard#haschangeSummary>

    Domain: 
        owl:Thing
    
    Range: 
        xsd:string
    
    
DataProperty: <http://ld.nice.org.uk/ns/qualitystandard#qs::hasDenominator>

    Domain: 
        <http://ld.nice.org.uk/ns/qualitystandard#QualityMeasure>
    
    Range: 
        xsd:string
    
    
DataProperty: <http://ld.nice.org.uk/ns/qualitystandard#qs::hasNumerator>

    Domain: 
        <http://ld.nice.org.uk/ns/qualitystandard#ProcessMeasure>
    
    Range: 
        xsd:string
    
    
DataProperty: <http://purl.org/dc/terms/abstract>

    Annotations: 
        rdfs:isDefinedBy <http://purl.org/dc/terms>,
        rdfs:comment "A summary of the resource."
    
    Domain: 
        owl:Thing
    
    Range: 
        xsd:string
    
    
DataProperty: <http://purl.org/dc/terms/date>

    
DataProperty: <http://purl.org/dc/terms/identifier>

    Annotations: 
        rdfs:comment "An unambiguous reference to the resource within a given context.",
        rdfs:isDefinedBy <http://purl.org/dc/terms>
    
    Domain: 
        <http://ld.nice.org.uk/ns/qualitystandard#Product>
    
    Range: 
        xsd:integer
    
    
DataProperty: <http://purl.org/dc/terms/title>

    Annotations: 
        rdfs:isDefinedBy "http://purl.org/dc/terms",
        rdfs:comment "A name given to the resource."
    
    Domain: 
        owl:Thing
    
    Range: 
        xsd:string
    
    
Class: <http://ld.nice.org.uk/ns/qualitystandard#ChangeEntry>

    SubClassOf: 
        <http://ld.nice.org.uk/ns/qualitystandard#TopLevelProvenanceConcept>,
        <http://ld.nice.org.uk/ns/qualitystandard#haschangeType> exactly 1 <http://ld.nice.org.uk/ns/qualitystandard#ChangeType>,
        <http://ld.nice.org.uk/ns/qualitystandard#haschangeDescription> some xsd:string,
        <http://ld.nice.org.uk/ns/qualitystandard#haschangeSummary> some xsd:string
    
    
Class: <http://ld.nice.org.uk/ns/qualitystandard#ChangeLog>

    SubClassOf: 
        <http://ld.nice.org.uk/ns/qualitystandard#TopLevelProvenanceConcept>,
        <http://ld.nice.org.uk/ns/qualitystandard#haschangeEntry> min 1 <http://ld.nice.org.uk/ns/qualitystandard#ChangeEntry>
    
    
Class: <http://ld.nice.org.uk/ns/qualitystandard#ChangeType>

    SubClassOf: 
        <http://ld.nice.org.uk/ns/qualitystandard#TopLevelProvenanceConcept>
    
    
Class: <http://ld.nice.org.uk/ns/qualitystandard#DevelopmentalQualityStatement>

    Annotations: 
        rdfs:comment "A developmental quality statement sets out an emergent area of cutting‑edge service delivery or technology currently found in a minority of providers and indicating outstanding performance. It will require specific, significant changes to be put in place, such as redesign of services or new equipment."
    
    SubClassOf: 
        <http://ld.nice.org.uk/ns/qualitystandard#QualityStatement>
    
    
Class: <http://ld.nice.org.uk/ns/qualitystandard#GuidanceStatus>

    Annotations: 
        rdfs:comment "The publication status of a NICE resource."
    
    
Class: <http://ld.nice.org.uk/ns/qualitystandard#MajorChange>

    SubClassOf: 
        <http://ld.nice.org.uk/ns/qualitystandard#ChangeType>
    
    DisjointWith: 
        <http://ld.nice.org.uk/ns/qualitystandard#MinorChange>
    
    
Class: <http://ld.nice.org.uk/ns/qualitystandard#MinorChange>

    SubClassOf: 
        <http://ld.nice.org.uk/ns/qualitystandard#ChangeType>
    
    DisjointWith: 
        <http://ld.nice.org.uk/ns/qualitystandard#MajorChange>
    
    
Class: <http://ld.nice.org.uk/ns/qualitystandard#OutcomeMeasure>

    Annotations: 
        rdfs:comment "An outcome measure addresses the outcome of care or service provision."
    
    SubClassOf: 
        <http://ld.nice.org.uk/ns/qualitystandard#QualityMeasure>
    
    DisjointWith: 
        <http://ld.nice.org.uk/ns/qualitystandard#ProcessMeasure>, <http://ld.nice.org.uk/ns/qualitystandard#StructureMeasure>
    
    
Class: <http://ld.nice.org.uk/ns/qualitystandard#PlaceholderStatement>

    Annotations: 
        rdfs:comment "A placeholder statement is an area of care that has been prioritised by the Quality Standards Advisory Committee but for which no source guidance is currently available. A placeholder statement indicates the need for evidence‑based guidance to be developed in this area."
    
    
Class: <http://ld.nice.org.uk/ns/qualitystandard#PopulationSpecifier>

    Annotations: 
        rdfs:comment "A class of facets by which a target population can be specified."
    
    
Class: <http://ld.nice.org.uk/ns/qualitystandard#ProcessMeasure>

    Annotations: 
        rdfs:comment "A process measure addresses the process of care or service provision"
    
    SubClassOf: 
        <http://ld.nice.org.uk/ns/qualitystandard#QualityMeasure>
    
    DisjointWith: 
        <http://ld.nice.org.uk/ns/qualitystandard#OutcomeMeasure>, <http://ld.nice.org.uk/ns/qualitystandard#StructureMeasure>
    
    
Class: <http://ld.nice.org.uk/ns/qualitystandard#Product>

    
Class: <http://ld.nice.org.uk/ns/qualitystandard#Published>

    Annotations: 
        rdfs:comment "Status of a resource that has been published and has not been withdrawn (still valid)."
    
    SubClassOf: 
        <http://ld.nice.org.uk/ns/qualitystandard#GuidanceStatus>,
        <http://ld.nice.org.uk/ns/qualitystandard#dateIssued> some xsd:dateTime,
        <http://ld.nice.org.uk/ns/qualitystandard#dateWithdrawn> max 0 xsd:dateTime
    
    DisjointWith: 
        <http://ld.nice.org.uk/ns/qualitystandard#Withdrawn>
    
    
Class: <http://ld.nice.org.uk/ns/qualitystandard#QualityMeasure>

    Annotations: 
        rdfs:comment "Quality measures are used to assess the quality of care or service provision specified in the quality statement."
    
    
Class: <http://ld.nice.org.uk/ns/qualitystandard#QualityStandard>

    Annotations: 
        rdfs:comment "NICE quality standards are concise sets of prioritised  quality statements designed to drive measurable quality improvements within a particular area of health or care."
    
    SubClassOf: 
        <http://ld.nice.org.uk/ns/qualitystandard#Product>,
        <http://ld.nice.org.uk/ns/qualitystandard#hasPart> some <http://ld.nice.org.uk/ns/qualitystandard#QualityStatement>
    
    DisjointWith: 
        <http://ld.nice.org.uk/ns/qualitystandard#QualityStatement>
    
    
Class: <http://ld.nice.org.uk/ns/qualitystandard#QualityStatement>

    Annotations: 
        rdfs:comment "A NICE Quality statement is a clear, measurable and concise statement to describe ‘enhanced practice’, which is both aspirational and achievable."
    
    SubClassOf: 
        <http://ld.nice.org.uk/ns/qualitystandard#Product>,
        <http://ld.nice.org.uk/ns/qualitystandard#partOf> some <http://ld.nice.org.uk/ns/qualitystandard#QualityStandard>
    
    DisjointWith: 
        <http://ld.nice.org.uk/ns/qualitystandard#QualityStandard>
    
    
Class: <http://ld.nice.org.uk/ns/qualitystandard#StructureMeasure>

    Annotations: 
        rdfs:comment "A  structure measure addresses the structure of care or services."
    
    SubClassOf: 
        <http://ld.nice.org.uk/ns/qualitystandard#QualityMeasure>
    
    DisjointWith: 
        <http://ld.nice.org.uk/ns/qualitystandard#OutcomeMeasure>, <http://ld.nice.org.uk/ns/qualitystandard#ProcessMeasure>
    
    
Class: <http://ld.nice.org.uk/ns/qualitystandard#TopLevelProvenanceConcept>

    
Class: <http://ld.nice.org.uk/ns/qualitystandard#Withdrawn>

    Annotations: 
        rdfs:comment "Status of a resource that thas been withdrawn after some time when it was a valid, published resource. No longer valid."
    
    SubClassOf: 
        <http://ld.nice.org.uk/ns/qualitystandard#GuidanceStatus>,
        <http://ld.nice.org.uk/ns/qualitystandard#dateWithdrawn> some xsd:dateTime
    
    DisjointWith: 
        <http://ld.nice.org.uk/ns/qualitystandard#Published>
    
    
Class: agegroup:AgeGroup

    Annotations: 
        rdfs:comment "List of age groups to support population definition."
    
    SubClassOf: 
        <http://ld.nice.org.uk/ns/qualitystandard#PopulationSpecifier>
    
    
Class: conditionordisease:ConditionOrDisease

    Annotations: 
        rdfs:comment "Class of conditions and diseases for population specification. Top level based on NICE Browse taxonomy structure. Mapping to equivalent SNOMED code where possible. Used for medical and mental health conditions."
    
    SubClassOf: 
        <http://ld.nice.org.uk/ns/qualitystandard#PopulationSpecifier>
    
    
Class: lifestylecondition:LifestyleCondition

    Annotations: 
        rdfs:comment "Conditions which have associated lifestyle factors, to include drug abuse, alcohol abuse and diet and physical activity related conditions."
    
    SubClassOf: 
        <http://ld.nice.org.uk/ns/qualitystandard#PopulationSpecifier>
    
    
Class: owl:Thing

    
Class: pico:Population

    Annotations: 
        rdfs:comment "Defined by at least one of the age, gender, ethnicity, disease, lifestyle condition concepts."
    
    EquivalentTo: 
        <http://ld.nice.org.uk/ns/qualitystandard#isSpecifiedBy> min 1 <http://ld.nice.org.uk/ns/qualitystandard#PopulationSpecifier>
    
    
Class: servicearea:ServiceArea

    Annotations: 
        rdfs:comment "Health or care service area to which a NICE quality statement is applicable."
    
    
Class: setting:Setting

    Annotations: 
        rdfs:comment "Physical setting  to which NICE quality statement is applicable."
    
    
